proofs/x86-64/avx2/ml_dsa_65/mldsa_65_prelude.ec
@@ -1,0 +1,54 @@
+require import AllCore List IntDiv RealExp StdBigop.
+
+from Spec require import GFq Rq Serialization Conversion Parameters VecMat MLDSA_W32_Rep.
+
+from JazzEC require import Array1280 Array640 Array1536 Array768 Array256 Array128 Array3200.
+
+import LArray KArray.
+
+axiom mldsa65_lvec: lvec = 5.
+axiom mldsa65_kvec: kvec = 6.
+axiom mldsa65_w_hint : w_hint = 55.
+axiom mldsa65_lambda : lambda = 192.
+axiom mldsa65_gamma1 : gamma1 = 524288. (* 2**19 *) 
+
+
+
+op  lvec_unflatten640(a : 'a Array3200.t) =
+     LArray.init (fun i => Array640.of_list witness (sub a (640*i) 640)).
+op  lvec_unflatten256(a : 'a Array1280.t) =
+     LArray.init (fun i => Array256.of_list witness (sub a (256*i) 256)).
+op  lvec_unflatten128(a : 'a Array640.t) =
+     LArray.init (fun i => Array128.of_list witness (sub a (128*i) 128)).
+
+op  kvec_unflatten256(a : 'a Array1536.t) =
+     KArray.init (fun i => Array256.of_list witness (sub a (256*i) 256)).
+op  kvec_unflatten128(a : 'a Array768.t) =
+     KArray.init (fun i => Array128.of_list witness (sub a (128*i) 128)).
+
+lemma kvec_unflatten256E i j (h : 'a Array1536.t) (P : 'a -> bool) :
+   0 <= i < kvec =>
+   0 <= j < 256 =>
+        all (all P) (kvec_unflatten256 h) =>
+        P h.[i*256+j].
+have eq_kvec := mldsa65_kvec.
+move => ??;rewrite allP => Hii. 
+have := Hii i _;1:smt().
+rewrite allP => Hjj. 
+have := Hjj j _;1:smt().
+by rewrite initiE 1:/# /= get_of_list 1:/# /= nth_sub /#. 
+qed.
+
+lemma kvec_unflatten256P i j (h1 : 'a Array1536.t) (h2 : ('b Array256.t) KArray.t) (F : 'a -> 'b) :
+   0 <= i < kvec =>
+   0 <= j < 256 =>
+        map (map F) (kvec_unflatten256 h1) = h2 =>
+        F h1.[i*256+j] = h2.[i].[j].
+have eq_kvec := mldsa65_kvec.
+move => ??; rewrite tP => Hii.
+have := Hii i _; 1:smt().
+rewrite tP => Hjj.
+have := Hjj j _; 1:smt().
+rewrite mapiE 1:/# /= mapiE 1:/# /= initiE 1:/# initiE 1:/# /=.
+by rewrite  /= !nth_sub /#. 
+qed.
